Weidenbach_Book/IsaSAT/IsaSAT_Print_LLVM.thy
@@ -11,17 +11,17 @@ definition print_confl :: \<open>64 word \<Rightarrow> unit\<close> where
 definition print_dec :: \<open>64 word \<Rightarrow> unit\<close> where
   \<open>print_dec _ = ()\<close>
 
-definition print_res :: \<open>64 word \<Rightarrow> unit\<close> where
-  \<open>print_res _ = ()\<close>
+definition print_res :: \<open>64 word \<Rightarrow> 64 word \<Rightarrow> unit\<close> where
+  \<open>print_res _ _ = ()\<close>
 
-definition print_lres :: \<open>64 word \<Rightarrow> unit\<close> where
-  \<open>print_lres _ = ()\<close>
+definition print_lres :: \<open>64 word \<Rightarrow> 64 word \<Rightarrow> unit\<close> where
+  \<open>print_lres _ _ = ()\<close>
 
 definition print_uset :: \<open>64 word \<Rightarrow> unit\<close> where
   \<open>print_uset _ = ()\<close>
 
-definition print_gcs :: \<open>64 word \<Rightarrow> unit\<close> where
-  \<open>print_gcs _ = ()\<close>
+definition print_gcs :: \<open>64 word \<Rightarrow> 64 word \<Rightarrow> unit\<close> where
+  \<open>print_gcs _ _ = ()\<close>
 
 definition print_binary_unit :: \<open>64 word \<Rightarrow> unit\<close> where
   \<open>print_binary_unit _ = ()\<close>
@@ -32,14 +32,14 @@ definition print_binary_red_removed :: \<open>64 word \<Rightarrow> unit\<close>
 definition print_purelit_elim :: \<open>64 word \<Rightarrow> unit\<close> where
   \<open>print_purelit_elim _ = ()\<close>
 
-definition print_purelit_rounds :: \<open>64 word \<Rightarrow> unit\<close> where
-  \<open>print_purelit_rounds _ = ()\<close>
+definition print_purelit_rounds :: \<open>64 word \<Rightarrow> 64 word \<Rightarrow> unit\<close> where
+  \<open>print_purelit_rounds _ _ = ()\<close>
 
 definition print_lbds :: \<open>64 word \<Rightarrow> unit\<close> where
   \<open>print_lbds _ = ()\<close>
 
-definition print_forward_rounds :: \<open>64 word \<Rightarrow> unit\<close> where
-  \<open>print_forward_rounds _ = ()\<close>
+definition print_forward_rounds :: \<open>64 word \<Rightarrow> 64 word \<Rightarrow> unit\<close> where
+  \<open>print_forward_rounds _ _ = ()\<close>
 
 definition print_forward_subsumed :: \<open>64 word \<Rightarrow> 64 word \<Rightarrow> unit\<close> where
   \<open>print_forward_subsumed _ _ = ()\<close>
@@ -69,14 +69,14 @@ sepref_def print_dec_impl
   by sepref
 
 sepref_def print_res_impl
-  is \<open>RETURN o print_res\<close>
-  :: \<open>word_assn\<^sup>k \<rightarrow>\<^sub>a unit_assn\<close>
+  is \<open>uncurry (RETURN oo print_res)\<close>
+  :: \<open>word_assn\<^sup>k *\<^sub>a word_assn\<^sup>k \<rightarrow>\<^sub>a unit_assn\<close>
   unfolding print_res_def
   by sepref
 
 sepref_def print_lres_impl
-  is \<open>RETURN o print_lres\<close>
-  :: \<open>word_assn\<^sup>k \<rightarrow>\<^sub>a unit_assn\<close>
+  is \<open>uncurry (RETURN oo print_lres)\<close>
+  :: \<open>word_assn\<^sup>k *\<^sub>a word_assn\<^sup>k \<rightarrow>\<^sub>a unit_assn\<close>
   unfolding print_lres_def
   by sepref
 
@@ -90,8 +90,8 @@ definition print_irred_clss :: \<open>64 word \<Rightarrow> unit\<close> where
   \<open>print_irred_clss _ = ()\<close>
 
 sepref_def print_gc_impl
-  is \<open>RETURN o print_gcs\<close>
-  :: \<open>word_assn\<^sup>k \<rightarrow>\<^sub>a unit_assn\<close>
+  is \<open>uncurry (RETURN oo print_gcs)\<close>
+  :: \<open>word_assn\<^sup>k *\<^sub>a word_assn\<^sup>k \<rightarrow>\<^sub>a unit_assn\<close>
   unfolding print_gcs_def
   by sepref
 
@@ -108,8 +108,8 @@ sepref_def print_binary_unit_impl
   by sepref
 
 sepref_def print_purelit_rounds_impl
-  is \<open>RETURN o print_purelit_rounds\<close>
-  :: \<open>word_assn\<^sup>k \<rightarrow>\<^sub>a unit_assn\<close>
+  is \<open>uncurry (RETURN oo print_purelit_rounds)\<close>
+  :: \<open>word_assn\<^sup>k *\<^sub>a word_assn\<^sup>k \<rightarrow>\<^sub>a unit_assn\<close>
   unfolding print_purelit_rounds_def
   by sepref
 
@@ -126,8 +126,8 @@ sepref_def print_binary_red_removed_impl
   by sepref
 
 sepref_def print_forward_rounds_impl
-  is \<open>RETURN o print_forward_rounds\<close>
-  :: \<open>word_assn\<^sup>k \<rightarrow>\<^sub>a unit_assn\<close>
+  is \<open>uncurry (RETURN oo print_forward_rounds)\<close>
+  :: \<open>word_assn\<^sup>k *\<^sub>a word_assn\<^sup>k \<rightarrow>\<^sub>a unit_assn\<close>
   unfolding print_forward_rounds_def
   by sepref
 
